MyProject/repr.lean
@@ -1,0 +1,33 @@
+-- repr.lean
+-- Description:
+-- - Allows us to verify the correctness of the gossip representation by viewing the state.
+
+import Mathlib.Data.Fin.Basic
+
+def ReprState (n : Nat) : Type := Fin n → Fin n → Bool
+
+def initialReprState (n : Nat) : ReprState n := fun i j => i = j
+
+def Call (n : Nat) := Fin n × Fin n
+
+def makeCall (s : ReprState n) : Call n → ReprState n
+  | (i, j), x, y =>
+    if x = i
+    then s x y ∨ s j y
+    else
+      if x = j
+        then s x y ∨ s i y
+        else s x y
+
+def makeCalls (s : ReprState n) (cs : List (Fin n × Fin n)) : ReprState n :=
+  cs.foldl makeCall s
+
+instance : Repr (ReprState n) := Repr.mk $
+  fun s _ =>
+    let whatIknows i := (i, ((Fin.list n).filter (s i)))
+    repr ((Fin.list n).map whatIknows)
+
+def calls : List (Fin 4 × Fin 4) := [(1, 2), (2, 3), (3, 0), (0, 1)]
+#eval repr (initialReprState 4)
+#eval repr (makeCall (initialReprState 4) (1, 3))
+#eval repr (makeCalls (initialReprState 4) calls)
